\documentclass[11pt]{article}
    %	options include 12pt or 11pt or 10pt
    %	classes include article, report, book, letter, thesis
    
    \usepackage{amsmath}
    \usepackage{array}
    \setlength\extrarowheight{2pt}
    \usepackage{graphicx}
    \graphicspath{ {/home/shanedrafahl/coms331/hw0} }
    
    \title{HW1}
    \author{Shane Drafahl}
    \date{30 August,2017}
    
    \begin{document}
    \maketitle
    
    1. Use mathematical induction to prove the following statements
    $ \newline \newline $
    (a)
    $ \newline $
    $ \forall_{n} \geq 1 $, $ \sum_{i = 1}^{n} i^{3} $ = $ ( \sum_{i = 1}^{n} i )^{2} $
    $ \newline \newline $
    $ \newline $
    lemma: $ \sum_{i = 1}^{n} i $ = $ \frac{n^{2}}{2} $ + $ \frac{n}{2} $ where $ n \in \mathbb{N} $
    $ \newline $
    Base Case: $ \sum_{i = 1}^{1} i $ = 1 = $ \frac{1^{2}}{2} $ + $ \frac{1}{2} $ 
    $ \newline $
    Inductive Hypothesis: $ \sum_{i = 1}^{n} i $ = $ \frac{n^{2}}{2} $ + $ \frac{n}{2} $ 
    $ \newline $
    Inductive Steps: 
    $ \newline $
    Using induction on n
    $ \newline $
    $ \frac{(n + 1)^{2}}{2} + \frac{n + 1}{2} $ = $ \frac{n^{2}}{2} $ + $ \frac{3n}{2} $ + 1 =
    $ \frac{n^{2}}{2} + \frac{n}{2} $ + $ (n + 1) $
    $ \newline \newline $
    So therefore the lemma is true for all natural numbers n greater than 1. 
    $ \newline \newline $    
    With the lemma we can solve the proof easier
    $ \newline \newline $
    Base Case: For n = 1 would be $ \sum_{i = 1}^{1} i^{3} $ = $ 1^{3} $ = 1.
    $ ( \sum_{i = 1}^{1} i )^{2} $ = 1. 
    $ \newline \newline $
    Inductive Hypothesis: From the base n is true for 
    $ \forall_{n} \geq 1 $, $ \sum_{i = 1}^{n} i^{3} $ = $ ( \sum_{i = 1}^{n} i )^{2} $
    $ \newline \newline $
    Inductive Step: Using lemma we can re-write this to 
    $ (\frac{n^{2}}{2}  +  \frac{n}{2})^{2} $ = $ \sum_{i = 1}^{n} i^{3} $
    We will first add n+1, $( \frac{(n + 1)^{2}}{2}  +  \frac{(n + 1)}{2})^{2} $ = $ \frac{n^{4}}{4} $ +
    $ \frac{3n^{3}}{2} $ + $ \frac{13n^{2}}{4} $ + 3n + 1 .
    Now we will do $ ( \frac{n^{2}}{2}  +  \frac{n}{2})^{2} $ + $ (n + 1)^{3} $ = 
    $ \frac{n^{4}}{4} $ +
    $ \frac{3n^{3}}{2} $ + $ \frac{13n^{2}}{4} $ + 3n + 1 . So therfore 
    $ \forall_{n} \geq 1 $, $ \sum_{i = 1}^{n} i^{3} $ = $ ( \sum_{i = 1}^{n} i )^{2} $
    is true for all natural numbers for n greater than or equal to 1.
    $ \newline \newline $
    (b) $ \forall_{n} \geq 4$, $ 2^{n} < n!$
    $ \newline \newline $

    \end{document}